src/arch/x64/X64.Taint_Semantics_s.fst
@@ -38,8 +38,11 @@ let extract_operands (i:ins) : (list operand * list operand) =
   | Add64 dst src -> [dst], [dst; src]
   | AddLea64 dst src1 src2 -> [dst], [dst; src1; src2]
   | AddCarry64 dst src -> [dst], [dst; src]
+  | Adcx64 dst src -> [dst], [dst; src]
+  | Adox64 dst src -> [dst], [dst; src]
   | Sub64 dst src -> [dst], [dst; src]
   | Mul64 src -> [OReg Rax; OReg Rdx], [OReg Rax; src]
+  | Mulx64 dst_hi dst_lo src -> [dst_hi; dst_lo], [OReg Rdx; src]
   | IMul64 dst src -> [dst], [dst; src]
   | Xor64 dst src -> [dst], [dst; src]
   | And64 dst src -> [dst], [dst; src]
@@ -98,7 +101,16 @@ let taint_eval_ins (ins:tainted_ins) (ts: traceState) : traceState =
   let t = ins.t in
   let i, dsts, srcs = ins.ops in
   let s = run (check (taint_match_list srcs t ts.memTaint)) ts.state in
-  let memTaint = update_taint_list ts.memTaint dsts t s in
+  let memTaint =
+    if Mulx64? i then
+    begin
+    let Mulx64 dst_hi dst_lo src = i in
+    let lo = FStar.UInt.mul_mod #64 (eval_reg Rdx s) (eval_operand src s) in
+    let s' = update_operand_preserve_flags' dst_lo lo s in
+    let memTaint = update_taint ts.memTaint dst_lo t s in
+    update_taint memTaint dst_hi t s'
+    end
+    else update_taint_list ts.memTaint dsts t s in
   (* Execute the instruction *)
   let s = run (eval_ins i) s in
   {state = s; trace = ts.trace; memTaint = memTaint}
